src/tls/Model.AEAD.fst
@@ -13,23 +13,42 @@ module MDM = FStar.Monotonic.DependentMap
 
 noextract
 inline_for_extraction
-let entry (a: SC.supported_alg): Tot eqtype =
+let entry_key (a: SC.supported_alg): Tot eqtype =
   [@inline_let]
   let t = SC.iv a in
   Crypto.Util.IntCast.seq_sec8_has_eq ();
   t
 
-let table
+noextract
+inline_for_extraction
+let entry_value
   (a: SC.supported_alg)
-  (kv: SC.kv a)
+  (phi: plain_pred)
+  (iv: entry_key a)
+: Tot Type0
+= (cipher: SC.cipher a & (plain: SC.decrypted cipher { phi plain }))
+
+noextract
+inline_for_extraction
+let table_inv
+  (a: SC.supported_alg)
+  (phi: plain_pred)
+  (map: FStar.DependentMap.t (entry_key a) (MDM.opt (entry_value a phi)))
+: Tot Type0
+= True
+
+let table
+  (r: HST.erid)
+  (a: SC.supported_alg)
   (phi: plain_pred)
 : Tot Type0
-= MDM.t HS.root (entry a) (fun iv -> (cipher: SC.cipher a & (plain: SC.decrypted cipher { phi plain }))) (fun _ -> True)
+= MDM.t r (entry_key a) (entry_value a phi) (table_inv a phi)
 
 noeq
 type state (a: SC.supported_alg) (phi: plain_pred) = {
   kv: SC.kv a;
-  table: (if F.ideal_iv then table a kv phi else unit)
+  region: (if F.ideal_iv then HST.erid else unit);
+  table: (if F.ideal_iv then table (region <: HST.erid) a phi else unit)
 }
 
 let state_kv
@@ -38,18 +57,22 @@ let state_kv
 : Tot (SC.kv a)
 = s.kv
 
+let state_region
+  (#a: SC.supported_alg) (#phi: plain_pred)
+  (s: state a phi {Flags.ideal_iv == true} )
+: Tot HST.erid
+= s.region
+
 let state_table
   (#a: SC.supported_alg) (#phi: plain_pred)
-  (s: state a phi)
-: Pure (table a (state_kv s) phi)
-  (requires (Flags.ideal_iv == true))
-  (ensures (fun _ -> True))
-= s.table <: table a (state_kv s) phi
+  (s: state a phi {Flags.ideal_iv == true})
+: Tot (table (state_region s) a phi)
+= s.table <: table (state_region s) a phi
 
 let invariant (#a: SC.supported_alg) (#phi: plain_pred) (h: HS.mem) (s: state a phi) : GTot Type0 =
   if F.ideal_iv
   then
-    h `HS.contains` state_table s
+    h `HS.contains` state_table s /\ HS.is_mm (state_table s)
   else
     True
 
@@ -57,7 +80,7 @@ let footprint
   #a #phi s
 = if F.ideal_iv
   then
-    B.loc_mreference (state_table s)
+    B.loc_freed_mreference (state_table s)
   else
     B.loc_none
 
@@ -115,3 +138,21 @@ let decrypt
     match SC.decrypt (state_kv s) iv Seq.empty cipher with
     | None -> None
     | Some plain -> Some plain
+
+let create
+  r #a k phi
+= if F.ideal_iv
+  then begin
+    HST.recall_region r;
+    HST.witness_region r;
+    let tbl : table r a phi = MDM.alloc #(entry_key a) #(entry_value a phi) #(table_inv a phi) #r () in
+    assume (HS.is_mm tbl); // TODO: fix FStar.Monotonic.DependentMap interface; implementation uses ralloc as expected
+    {kv = k; region = r; table = tbl}
+  end else
+    {kv = k; region = (); table = ()}
+
+let free
+  #a #phi s
+= if F.ideal_iv
+  then HST.rfree (state_table s)
+  else ()
